Move to language level annotations

Atomics.thy
@@ -21,10 +21,6 @@ text \<open>Weakest precondition for a precondition and postrelation\<close>
 definition wp 
   where "wp pre post Q \<equiv> pre \<inter> {m. (\<forall>m'. (m,m') \<in> post \<longrightarrow> m' \<in> Q)}"
 
-text \<open>Weakest precondition of the transitive closure of an arbitrary state relation\<close>
-abbreviation wp\<^sub>t :: "'b rpred \<Rightarrow> 'b pred \<Rightarrow> 'b pred"
-  where "wp\<^sub>t R P \<equiv> wp (UNIV) (R\<^sup>*) P"
-
 subsection \<open>Helper Lemmas\<close>
 
 lemma stable_conseqI [intro]:
@@ -43,29 +39,21 @@ lemma stable_transitive:
   using assms by (induct rule: rtrancl.induct) (auto simp: stable_def)
 
 lemma stable_wp\<^sub>tI:
-  "stable R P \<Longrightarrow> P \<subseteq> wp\<^sub>t R P"
+  "stable R P \<Longrightarrow> P \<subseteq> wp UNIV (R\<^sup>* ) P"
   unfolding wp_def using stable_transitive by fast
 
 section \<open>Atomic Properties\<close>
 
-locale atomics =
-  fixes behv :: "'a \<Rightarrow> 'b rel" 
-  and vc :: "'a \<Rightarrow> 'b set"
-
-context atomics
-begin
-
 text \<open>Weakest precondition of a basic instruction, based on the locale's 
       verification conditions and behaviours.\<close>
-abbreviation wp\<^sub>\<alpha> :: "'a \<Rightarrow> 'b set \<Rightarrow> 'b set"
-  where "wp\<^sub>\<alpha> \<alpha> Q \<equiv> wp (vc \<alpha>) (behv \<alpha>) Q"
+abbreviation wp\<^sub>\<alpha> :: "('a,'b) inst \<Rightarrow> 'a set \<Rightarrow> 'a set"
+  where "wp\<^sub>\<alpha> \<alpha> Q \<equiv> wp (vc \<alpha>) (beh \<alpha>) Q"
 
 text \<open>Weakest precondition of a program, only covering basic instructions, environment steps and 
       sequential composition as these are sufficient for the logic's checks.\<close>
-fun wp\<^sub>c :: "('a,'b) com \<Rightarrow> 'b set \<Rightarrow> 'b set"
+fun wp\<^sub>c :: "('a,'b) com \<Rightarrow> 'a set \<Rightarrow> 'a set"
   where 
     "wp\<^sub>c (Basic \<alpha>) Q = wp\<^sub>\<alpha> \<alpha> Q" |
-    "wp\<^sub>c (Env r) Q = wp\<^sub>t r Q" |
     "wp\<^sub>c (c\<^sub>1 ; c\<^sub>2) Q = wp\<^sub>c c\<^sub>1 (wp\<^sub>c c\<^sub>2 Q)" |
     "wp\<^sub>c _ Q = undefined"
 
@@ -74,24 +62,17 @@ definition refine :: "('a,'b) com \<Rightarrow> ('a,'b) com \<Rightarrow> bool" 
   where "c \<sqsubseteq> c' \<equiv> \<forall>Q. wp\<^sub>c c Q \<subseteq> wp\<^sub>c c' Q"
 
 text \<open>Merge the verification condition and behaviour to define evaluation\<close>
-definition eval :: "'a \<Rightarrow> 'b rpred"
-  where "eval \<alpha> \<equiv> {(m,m'). m \<in> vc \<alpha> \<longrightarrow> (m,m') \<in> behv \<alpha>}"
+definition eval :: "('a,'b) inst \<Rightarrow> 'a rpred"
+  where "eval \<alpha> \<equiv> {(m,m'). m \<in> vc \<alpha> \<longrightarrow> (m,m') \<in> beh \<alpha>}"
 
 text \<open>Specification check, ensuring an instruction conforms to a relation\<close>
-abbreviation guar :: "'a \<Rightarrow> 'b rpred \<Rightarrow> bool"
-  where "guar \<alpha> G \<equiv> {(m,m'). m \<in> vc \<alpha>} \<inter> behv \<alpha> \<subseteq> G"
-
-end
+abbreviation guar :: "('a,'b) inst \<Rightarrow> 'a rpred \<Rightarrow> bool"
+  where "guar \<alpha> G \<equiv> {(m,m'). m \<in> vc \<alpha>} \<inter> beh \<alpha> \<subseteq> G"
 
 section \<open>Atomic Rule\<close>
 
-locale atomic_rules = atomics
-
-context atomic_rules
-begin
-
 text \<open>Rule for an atomic operation\<close>
-definition atomic_rule :: "'b rpred \<Rightarrow> 'b rpred \<Rightarrow> 'b pred \<Rightarrow> 'a \<Rightarrow> 'b pred \<Rightarrow> bool" 
+definition atomic_rule :: "'a rpred \<Rightarrow> 'a rpred \<Rightarrow> 'a pred \<Rightarrow> ('a,'b) inst \<Rightarrow> 'a pred \<Rightarrow> bool" 
   ("_,_ \<turnstile>\<^sub>A _ {_} _" [40,0,0,0,40] 40)
   where "R,G \<turnstile>\<^sub>A P {\<alpha>} Q \<equiv> P \<subseteq> wp\<^sub>\<alpha> \<alpha> Q \<and> guar \<alpha> G \<and> stable R P \<and> stable R Q"
 
@@ -116,7 +97,7 @@ lemma actomic_conjI [intro]:
   assumes "R,G \<turnstile>\<^sub>A P\<^sub>1 {\<alpha>} Q\<^sub>1" "R,G  \<turnstile>\<^sub>A P\<^sub>2 {\<alpha>} Q\<^sub>2"
   shows "R,G \<turnstile>\<^sub>A P\<^sub>1 \<inter> P\<^sub>2 {\<alpha>} Q\<^sub>1 \<inter> Q\<^sub>2"
   using assms unfolding atomic_rule_def wp_def stable_def
-  by (intro conjI) blast+
+  by fast
 
 text \<open>Add an invariant across an atomic judgement\<close>
 lemma atomic_frameI [intro]:
@@ -126,13 +107,11 @@ lemma atomic_frameI [intro]:
   unfolding atomic_rule_def
 proof (safe, goal_cases)
   case (1 x)
-  hence "{(m,m'). m \<in> P \<inter> vc \<alpha>} \<inter> behv \<alpha> \<subseteq> R\<^sub>2" "x \<in> vc \<alpha>"
+  hence "{(m,m'). m \<in> P \<inter> vc \<alpha>} \<inter> beh \<alpha> \<subseteq> R\<^sub>2" "x \<in> vc \<alpha>"
     using assms(1,3) by (auto simp: wp_def atomic_rule_def)
   hence "x \<in> wp\<^sub>\<alpha> \<alpha> M" using assms(2) 1 by (auto simp: wp_def stable_def)
   moreover have "x \<in> wp\<^sub>\<alpha> \<alpha> Q" using 1 assms(1) by (auto simp: atomic_rule_def wp_def)
   ultimately show ?case by (auto simp: wp_def)
 qed (insert assms, auto simp: atomic_rule_def wp_def)
-
-end
 
 end
