Interference.thy
@@ -9,8 +9,10 @@ Define the necessary side-conditions to ensure reordering cannot introduce inter
 First defines properties to avoid interference for the early execution of an instruction,
 and then defines all possible early executions that may be observed for a program.
 \<close>
-
-locale interference = semantics
+                         
+locale interference = semantics re fwd
+  for re :: "('a,'b) inst \<Rightarrow> ('a,'b) inst \<Rightarrow> bool" (infix "\<hookleftarrow>" 100)
+  and fwd :: "('a,'b) inst \<Rightarrow> ('a,'b) inst \<Rightarrow> ('a,'b) inst" ("_\<langle>_\<rangle>" [1000,0] 1000)
 
 context interference
 begin
@@ -21,7 +23,7 @@ text \<open>
 Independence of two instructions \<beta> and \<alpha> under environment R, 
 such that the early execution of \<alpha> is assumed to be possible and 
 cannot invalidate sequential reasoning.\<close>
-definition inter\<^sub>\<alpha> :: "'b rpred \<Rightarrow> 'b rpred \<Rightarrow> 'a \<Rightarrow> 'a \<Rightarrow> bool"
+definition inter\<^sub>\<alpha> :: "'a rpred \<Rightarrow> 'a rpred \<Rightarrow> ('a,'b) inst \<Rightarrow> ('a,'b) inst \<Rightarrow> bool"
   where "inter\<^sub>\<alpha> R G \<beta> \<alpha> \<equiv> 
           Env R ; Basic \<beta> ; Env R ; Basic \<alpha> \<sqsubseteq> Env R ; Basic \<alpha>\<langle>\<beta>\<rangle> ; Env R ; Basic \<beta> \<and>
           guar \<alpha>\<langle>\<beta>\<rangle> G"
@@ -31,26 +33,13 @@ Independence of program c and instruction \<alpha> under environment R,
 such that the early execution of \<alpha> is assumed to be possible and 
 cannot invalidate sequential reasoning.
 Define by recursively iterating over the program and capturing the forwarding throughout.\<close>
-fun inter\<^sub>c :: "'b rpred \<Rightarrow> 'b rpred \<Rightarrow> ('a,'b) com \<Rightarrow> 'a \<Rightarrow> bool"
+fun inter\<^sub>c :: "'a rpred \<Rightarrow> 'a rpred \<Rightarrow> ('a,'b) com \<Rightarrow> ('a,'b) inst \<Rightarrow> bool"
   where
     "inter\<^sub>c R G (Basic \<beta>) \<alpha> = inter\<^sub>\<alpha> R G \<beta> \<alpha>" |
     "inter\<^sub>c R G (c\<^sub>1 ; c\<^sub>2) \<alpha> = (inter\<^sub>c R G c\<^sub>1 \<alpha>\<llangle>c\<^sub>2\<rrangle> \<and> inter\<^sub>c R G c\<^sub>2 \<alpha>)" |
     "inter\<^sub>c R G (c\<^sub>1 \<sqinter> c\<^sub>2) \<alpha> = (inter\<^sub>c R G c\<^sub>1 \<alpha> \<and> inter\<^sub>c R G c\<^sub>2 \<alpha>)" |
     "inter\<^sub>c R G (c*) \<alpha> = inter\<^sub>c R G c \<alpha>" |
     "inter\<^sub>c R G _ \<alpha> = True"
-
-text \<open>
-Instrumented version of the semantics that collects the reordering effects.
-Given c \<mapsto>[\<alpha>,r,\<alpha>'] c', this corresponds to c \<mapsto>\<alpha> c', such that
-r should be the program \<alpha>' has to reorder with in c to execute and 
-\<alpha> should be \<alpha>' forwarded across r.\<close>
-inductive execute_collect :: "('a,'b) com \<Rightarrow> 'a \<Rightarrow> ('a,'b) com \<Rightarrow> 'a \<Rightarrow> ('a,'b) com \<Rightarrow> bool"
-  ("_ \<mapsto>[_,_,_] _" [71,0,0,0,71] 70)
-  where
-  act[intro]:  "Basic \<alpha> \<mapsto>[\<alpha>,Nil,\<alpha>] Nil" |
-  seq[intro]:  "c\<^sub>1 \<mapsto>[\<alpha>,c,\<alpha>'] c\<^sub>1' \<Longrightarrow> c\<^sub>1 ; c\<^sub>2 \<mapsto>[\<alpha>,c,\<alpha>'] c\<^sub>1' ; c\<^sub>2" |
-  ooo[intro]:  "c\<^sub>1 \<mapsto>[\<alpha>,c,\<alpha>'] c\<^sub>1' \<Longrightarrow> \<gamma> < c\<^sub>2 <\<^sub>c \<alpha> \<Longrightarrow> c\<^sub>2 ; c\<^sub>1 \<mapsto>[\<gamma>,c\<^sub>2;c,\<alpha>'] c\<^sub>2 ; c\<^sub>1'"
-inductive_cases execute_collect[elim]: "c\<^sub>1 \<mapsto>[\<alpha>,c,\<alpha>'] c\<^sub>1'"
 
 text \<open>Compute possible reorderings of the program using the instrumented semantics\<close>
 inductive reorder_trace
@@ -75,20 +64,11 @@ text \<open>Interference check is preserved across an execution step and prevent
 lemma indep_stepI [intro]:
   assumes "inter R G c" "c \<mapsto>[\<alpha>,r,\<alpha>'] c'"
   shows "inter R G c' \<and> inter\<^sub>c R G r \<alpha>'"
-  using assms reorder_trace.intros(1,3)
-  unfolding inter_def by force
-
-text \<open>Instrumented semantics collects valid reorderings\<close>
-lemma collect_reorder:
-  assumes "c \<mapsto>[\<alpha>',r,\<alpha>] c'"
-  shows "\<alpha>' < r <\<^sub>c \<alpha>"
-  using assms by (induct, auto)
-
-text \<open>Convert a normal execution step into an instrumented step\<close>
-lemma exec_collect:
-  assumes "c \<mapsto>\<^sub>\<alpha> c'" "local c"
-  shows "\<exists>r \<alpha>'. c \<mapsto>[\<alpha>,r,\<alpha>'] c'"
-  using assms by induct auto
+proof -
+  have "reorder_trace [(r, \<alpha>')] c" using assms reorder_trace.intros by simp
+  hence "inter\<^sub>c R G r \<alpha>'" using assms by (auto simp: inter_def)
+  thus ?thesis using assms reorder_trace.intros(3)[OF assms(2)] inter_def by force
+qed
 
 end
 
