Syntax.thy
@@ -4,6 +4,14 @@ begin
 
 chapter \<open>While Language Syntax\<close>
 
+type_synonym ('a,'b) inst = "'a set \<times> 'a rel \<times> 'b"
+
+abbreviation vc :: "('a,'b) inst \<Rightarrow> 'a set"
+  where "vc \<alpha> \<equiv> fst \<alpha>"
+
+abbreviation beh :: "('a,'b) inst \<Rightarrow> 'a rel"
+  where "beh \<alpha> \<equiv> fst (snd \<alpha>)"
+
 text \<open>
 A While language with non-deterministic choice, iteration and parallel composition.
 Also includes special commands for environment steps, which is useful for describing
@@ -11,8 +19,7 @@ refinement properties. These have no evaluation semantics or rules however.
 \<close>
 datatype ('a,'b) com =
   Nil
-  | Env "'b rel"
-  | Basic "'a"
+  | Basic "('a,'b) inst"
   | Seq "('a,'b) com" "('a,'b) com" (infixr ";" 80)
   | Choice "('a,'b) com" "('a,'b) com" (infixr "\<sqinter>" 150)
   | Loop "('a,'b) com" ("_*" [100] 150)
@@ -26,5 +33,8 @@ fun local :: "('a,'b) com \<Rightarrow> bool"
     "local (c\<^sub>1 \<sqinter> c\<^sub>2) = (local c\<^sub>1 \<and> local c\<^sub>2)" |  
     "local (c*) = (local c)" |    
     "local _ = True"
+
+abbreviation Env
+  where "Env R \<equiv> Basic (UNIV,R\<^sup>*,undefined)"
 
 end
